IsaSAT: add setup to print progress while running

Weidenbach_Book/IsaSAT_Show.thy
@@ -21,6 +21,10 @@ definition println_string :: \<open>String.literal \<Rightarrow> unit\<close> wh
 definition print_c :: \<open>64 word \<Rightarrow> unit\<close> where
   \<open>print_c _ = ()\<close>
 
+
+definition print_char :: \<open>64 word \<Rightarrow> unit\<close> where
+  \<open>print_char _ = ()\<close>
+
 definition print_uint64 :: \<open>64 word \<Rightarrow> unit\<close> where
   \<open>print_uint64 _ = ()\<close>
 
@@ -89,5 +93,43 @@ lemma isasat_current_status_id:
    \<langle>{(S, T). (S, T) \<in> twl_st_heur \<and> length (get_clauses_wl_heur S) \<le> r}\<rangle>nres_rel\<close>
   by (intro frefI nres_relI)
     (auto simp: twl_st_heur_def isasat_current_status_def)
+
+definition print_open_colour :: \<open>64 word \<Rightarrow> unit\<close> where
+  \<open>print_open_colour _ = ()\<close>
+
+definition print_close_colour :: \<open>64 word \<Rightarrow> unit\<close> where
+  \<open>print_close_colour _ = ()\<close>
+
+
+definition isasat_print_progress :: \<open>64 word \<Rightarrow> 64 word \<Rightarrow> stats \<Rightarrow> _ \<Rightarrow> unit\<close> where
+\<open>isasat_print_progress c curr_phase =
+   (\<lambda>(propa, confl, decs, frestarts, lrestarts, uset, gcs, lbds) lcount.
+     let
+         _ = print_c propa;
+         _ = if curr_phase = 1 then print_open_colour 33 else ();
+         _ = print_char c;
+         _ = print_uint64 propa;
+         _ = print_uint64 confl;
+         _ = print_uint64 frestarts;
+         _ = print_uint64 lrestarts;
+         _ = print_uint64 uset;
+         _ = print_uint64 gcs;
+         _ = print_uint64 lbds;
+         _ = print_close_colour 0
+     in
+       ())\<close>
+
+
+definition isasat_current_progress :: \<open>64 word \<Rightarrow> twl_st_wl_heur \<Rightarrow> unit nres\<close> where
+\<open>isasat_current_progress =
+   (\<lambda>c (M', N', D', j, W', vm, clvls, cach, lbd, outl, stats,
+       heur, avdom,
+       vdom, lcount, opts, old_arena).
+     let
+       curr_phase = current_restart_phase heur;
+       stats = print_current_information stats lcount;
+       _ = isasat_print_progress c curr_phase stats lcount
+     in RETURN ())\<close>
+
 
 end
