Weidenbach_Book/IsaSAT_Show_LLVM.thy
@@ -45,6 +45,17 @@ sepref_def isasat_current_information_impl [llvm_code]
 
 declare isasat_current_information_impl.refine[sepref_fr_rules]
 
+lemma current_restart_phase_alt_def:
+  \<open>current_restart_phase =
+    (\<lambda>(fast_ema, slow_ema, (ccount, ema_lvl, restart_phase, end_of_phase), wasted, \<phi>).
+      restart_phase)\<close>
+  by (auto intro!: ext)
+
+sepref_def current_restart_phase_impl
+  is \<open>RETURN o current_restart_phase\<close>
+  :: \<open>heuristic_assn\<^sup>k \<rightarrow>\<^sub>a word_assn\<close>
+  unfolding current_restart_phase_alt_def heuristic_assn_def
+  by sepref
 
 sepref_def isasat_current_status_fast_code
   is \<open>isasat_current_status\<close>
@@ -54,6 +65,40 @@ sepref_def isasat_current_status_fast_code
   unfolding fold_tuple_optimizations
   by sepref
 
-declare isasat_current_status_fast_code.refine[sepref_fr_rules]
+
+sepref_def print_open_colour_impl
+  is \<open>RETURN o print_open_colour\<close>
+  :: \<open>word_assn\<^sup>k \<rightarrow>\<^sub>a unit_assn\<close>
+  unfolding print_open_colour_def
+  by sepref
+
+
+sepref_def print_close_colour_impl
+  is \<open>RETURN o print_close_colour\<close>
+  :: \<open>word_assn\<^sup>k \<rightarrow>\<^sub>a unit_assn\<close>
+  unfolding print_close_colour_def
+  by sepref
+
+sepref_def print_char_impl
+  is \<open>RETURN o print_char\<close>
+  :: \<open>word_assn\<^sup>k \<rightarrow>\<^sub>a unit_assn\<close>
+  unfolding print_char_def
+  by sepref
+
+sepref_def isasat_print_progress_impl
+  is \<open>uncurry3 (RETURN oooo isasat_print_progress)\<close>
+  :: \<open>word_assn\<^sup>k *\<^sub>a word_assn\<^sup>k *\<^sub>a stats_assn\<^sup>k *\<^sub>a uint64_nat_assn\<^sup>k \<rightarrow>\<^sub>a unit_assn\<close>
+  unfolding isasat_print_progress_def
+  by sepref
+
+term isasat_current_progress
+
+sepref_def isasat_current_progress_impl
+  is \<open>uncurry isasat_current_progress\<close>
+  :: \<open>word_assn\<^sup>k *\<^sub>a isasat_bounded_assn\<^sup>k \<rightarrow>\<^sub>a unit_assn\<close>
+  supply [[goals_limit=1]]
+  unfolding isasat_bounded_assn_def isasat_current_progress_def
+  unfolding fold_tuple_optimizations
+  by sepref
 
 end
